bedrock2/src/bedrock2/FrameRule.v
@@ -16,7 +16,6 @@ Require Import Coq.Lists.List.
 Section semantics.
   Context {width: Z} {BW: Bitwidth width} {word: word.word width} {mem: map.map word byte}.
   Context {locals: map.map String.string word}.
-  Context {env: map.map String.string (list String.string * list String.string * cmd)}.
   Context {ext_spec: ExtSpec}.
   Context {mem_ok: map.ok mem} {word_ok: word.ok word}.
 
