bedrock2/src/bedrock2Examples/memmove.v
@@ -53,7 +53,6 @@ Section WithParameters.
 
 
   Context {word_ok: word.ok word} {mem_ok: map.ok mem} {locals_ok : map.ok locals}
-    {env : map.map string (list string * list string * Syntax.cmd)} {env_ok : map.ok env}
     {ext_spec_ok : ext_spec.ok ext_spec}.
 
   Import coqutil.Tactics.letexists coqutil.Tactics.Tactics coqutil.Tactics.autoforward.
